Hey there! Let's talk about solving an equation. Suppose we have the equation $$(2X - 1)(X + 4) = 0$$. Try to find the values of X that make this equation true. Take a moment to think about it and then we can solve it together.

Alright, let's break it down. You might want to multiply everything out, but there's an easier way. Notice that we have two things being multiplied together, and their product is zero. That means at least one of these things must be zero.

Let's say we have two numbers, A and B, and their product is zero: $A \cdot B = 0$. The only way this can happen is if A is zero, or B is zero, or both are zero. Think about it: if $A = 7$, B must be zero to make the product zero, and if $B = 5$, A must be zero. So for $A \cdot B = 0$, either A or B or both must be zero. This is super important and helps us solve the equation.

Now, let's use this idea for our equation. We can think of $2X - 1$ as A and $X + 4$ as B. So, either $2X - 1 = 0$ or $X + 4 = 0$ (or both).

Let's solve each one:
- For $2X - 1 = 0$: 
  $$2X - 1 = 0$$
  Add 1 to both sides:
  $$2X = 1$$
  Now divide by 2:
  $$X = \frac{1}{2}$$

- For $X + 4 = 0$:
  $$X + 4 = 0$$
  Subtract 4 from both sides:
  $$X = -4$$

So, our solutions are $X = \frac{1}{2}$ or $X = -4$. 

To check, plug $X = \frac{1}{2}$ back into the original equation. You'll see the product becomes zero because $2X - 1$ becomes zero. Similarly, if $X = -4$, the product becomes zero because $X + 4$ becomes zero.

Now, let's try another example that involves a function. Suppose someone gives you $$F(X) = (X - 5)(5X + 2)$$ and asks for the zeros of $F(X)$. This means we're looking for the values of X that make $F(X) = 0$.

So:
$$(X - 5)(5X + 2) = 0$$
Using our earlier logic, we set each expression to zero:
- $X - 5 = 0$: 
  $$X - 5 = 0$$
  Add 5 to both sides:
  $$X = 5$$

- $5X + 2 = 0$:
  $$5X + 2 = 0$$
  Subtract 2 from both sides:
  $$5X = -2$$
  Divide by 5:
  $$X = -\frac{2}{5}$$

So, the zeros of $F(X)$ are $X = 5$ and $X = -\frac{2}{5}$. 

If you substitute these back into the function, you'll see that they make the product zero, just like in the earlier problem.

I hope this makes things clearer! If you have any more questions or need further explanations, feel free to ask. Happy learning!