Hey there! Let's see if we can figure this Math problem out together. We're asked to find the value of:

$$ -2 \times f(-6) + g(1) $$

They've given us the functions, $$f(x)$$ and $$g(x)$$, using graphs. 

First, we need to find out what $$f(-6)$$ is. We're plugging $$-6$$ into the $$f(x)$$ function. If we look at the graph for $$f(x)$$, we see that when $$x = -6$$, $$f(x) = 7$$. So:

$$ f(-6) = 7 $$

Next, let's figure out what $$g(1)$$ is. We're plugging $$1$$ into the $$g(x)$$ function. Looking at the graph for $$g(x)$$, when $$x = 1$$, $$g(x) = -5$$. So:

$$ g(1) = -5 $$

Now, let's put it all together:

$$ -2 \times f(-6) + g(1) = -2 \times 7 + (-5) $$

First, we calculate:

$$ -2 \times 7 = -14 $$

Then, we add the $$-5$$ to $$-14$$:

$$ -14 + (-5) = -19 $$

So, the final answer is $$-19$$! And we're done! Great job following along! ðŸ’¡