Sure! Let's take a look at this math problem and solve it step-by-step. Hereâ€™s how it goes:

We start with the equation:
$$ \frac{3}{4}x + 2 = \frac{3}{8}x - 4 $$

Dealing with fractions can be tricky, so let's get rid of them by multiplying both sides of the equation by a number that makes the fractions whole numbers. The smallest number that both 4 and 8 can divide into is 8. So, we multiply everything by 8.

Let's see what happens when we do that:
- $$ 8 \times \frac{3}{4}x = 6x $$
- $$ 8 \times 2 = 16 $$
- $$ 8 \times \frac{3}{8}x = 3x $$
- $$ 8 \times -4 = -32 $$

This transforms our equation to:
$$ 6x + 16 = 3x - 32 $$

Next, we want to get all the $$x$$ terms on one side and the constant numbers on the other. To do that, let's subtract $$3x$$ from both sides:
$$ 6x - 3x + 16 = 3x - 3x - 32 $$

Simplifying that, we get:
$$ 3x + 16 = -32 $$

Now, let's get rid of the 16 on the left by subtracting 16 from both sides:
$$ 3x + 16 - 16 = -32 - 16 $$

This gives us:
$$ 3x = -48 $$

To solve for $$x$$, we divide both sides by 3:
$$ \frac{3x}{3} = \frac{-48}{3} $$

This simplifies to:
$$ x = -16 $$

So, our solution is $$ x = -16 $$. 

To make sure this works, let's plug $$ x = -16 $$ back into the original equation:

The left side:
$$ \frac{3}{4}(-16) + 2 = -12 + 2 = -10 $$

The right side:
$$ \frac{3}{8}(-16) - 4 = -6 - 4 = -10 $$

Both sides equal -10, so our solution $$ x = -16 $$ is correct!

Great job!