Sure! Let's break it down step by step.

First, we need to factor the expression $$25x^2 - 30x + 9$$. 

Notice that the leading number (coefficient) in front of $$x^2$$ isn't 1, and there doesn’t seem to be any common factors across all terms. Both 25 and 30 are divisible by 5, but 9 isn’t.

We could use grouping to factor this, but if we look closely, 25 is a perfect square, as is 25$$x^2$$ since it is $$(5x)^2$$. Similarly, 9 is a perfect square, as it is $$(3)^2$$ (and also $$( - 3)^2$$).

Perhaps this expression is a perfect square trinomial. When we have $$(ax + b)^2$$, expanding it gives:
$$(ax + b) \times (ax + b) = a^2x^2 + 2abx + b^2$$.

Let’s rewrite the given expression:
$$25x^2 - 30x + 9$$.

Here, $$a^2 = 25$$ and $$b^2 = 9$$, which means $$a$$ can be $$\pm 5$$ and $$b$$ can be $$\pm 3$$. 

Let's check the middle term:
$$2ab = -30$$. Dividing by 2, we get $$ab = -15$$.

This product should be negative, meaning one of these must be positive and the other negative. Since the product of 5 and 3 is 15, we should get the right combination by making one pair positive and the other negative.

We can choose $$a = 5$$ and $$b = -3$$ or $$a = -5$$ and $$b = 3$$. Both pairs will work.

So either:
$$5x - 3$$, which squared is $$(5x - 3)^2$$,

or

$$-5x + 3$$, which squared is $$( - 5x + 3)^2$$.

Both work because $$( -5x + 3)^2 = (-1)^2(5x - 3)^2 = (5x - 3)^2$$.

In the end, the factored form is:

$$(5x - 3)^2$$ or $$( - 5x + 3)^2$$.

Both are correct and give us the original expression when expanded.