Sure! Let's break it down together. 

We have the graph of an exponential function called \( m(x) \). We want to figure out what \( m(6) \) is. Give it a try first, then check back here.

Alright, let's think about this step by step. We know \( m(x) \) is an exponential function, which means it looks something like this: 
$$
m(x) = a \cdot r^x
$$ 
Here, \( a \) is the starting value, and \( r \) is the common ratio.

First, we find the starting value, \( a \), by looking at the graph when \( x = 0 \). At \( x = 0 \), \( m(x) = 9 \). So, \( a = 9 \).

Next, we need to find the common ratio, \( r \). Let's use a small table to help us. 

\[ 
\begin{array}{|c|c|} 
\hline
x & m(x) \\ 
\hline
0 & 9 \\ 
\hline
1 & 3 \\ 
\hline
\end{array} 
\]

From the table, when \( x \) goes from 0 to 1, \( m(x) \) goes from 9 to 3. To find \( r \), we see what we multiplied by to go from 9 to 3. 

$$
r = \frac{3}{9} = \frac{1}{3}
$$ 

Now, we have our initial value \( a = 9 \) and our common ratio \( r = \frac{1}{3} \). So, our function looks like this: 
$$
m(x) = 9 \cdot \left(\frac{1}{3}\right)^x
$$ 

But we want to find \( m(6) \).

$$
m(6) = 9 \cdot \left(\frac{1}{3}\right)^6
$$ 

Now, let's calculate \( \left(\frac{1}{3}\right)^6 \). 

$$
\left(\frac{1}{3}\right)^6 = \frac{1^6}{3^6} = \frac{1}{729}
$$ 

So now we have:

$$
m(6) = 9 \cdot \frac{1}{729}
$$ 

We can simplify this by recognizing that:

$$
9 = 3^2
$$ 

So we can write:

$$
m(6) = \frac{3^2}{3^6} = 3^{2-6} = 3^{-4} = \frac{1}{3^4}
$$ 

And calculating \( 3^4 \):

$$
3^4 = 81
$$ 

So, 

$$
m(6) = \frac{1}{81}
$$ 

Therefore, \( m(6) = \frac{1}{81} \).

We could also check our answer by continuing our table all the way to 6 if you like: 
\[ 
\begin{array}{|c|c|} 
\hline
x & m(x) \\ 
\hline
0 & 9 \\ 
\hline
1 & 3 \\ 
\hline
2 & 1 \\ 
\hline
3 & \frac{1}{3} \\ 
\hline
4 & \frac{1}{9} \\ 
\hline
5 & \frac{1}{27} \\ 
\hline
6 & \frac{1}{81} \\ 
\hline
\end{array} 
\]

This confirms that \( m(6) = \frac{1}{81} \). Great job!