Hey there! Let's take a look at how to graph the equation $$y = -2 \cdot (x - 2)^2 + 5$$ together. I'll break it down step-by-step for you.

First, let's write the equation down again:
$$y = -2 \cdot (x - 2)^2 + 5$$

One important thing to notice is that the term $$(x - 2)^2$$ is always non-negative (it means it can be zero or positive but never negative). Since it's squared, it's never going to be negative.

When we multiply this squared term by -2, the value becomes non-positive (zero or negative). So this part, $$-2 \cdot (x - 2)^2$$, is always less than or equal to zero.

This means the maximum value that $$y$$ can have is when $$-2 \cdot (x - 2)^2$$ is equal to zero. And when this happens, $$y$$ will be equal to 5.

So, if we find when $$(x - 2)^2$$ equals zero, we know that's when $$y$$ is at its maximum. $$(x - 2)^2$$ is zero when $$x = 2$$. So, the point $$(2, 5)$$ is the highest point on the graph of the parabola. This point is called the vertex.

Let's plot this vertex:
- The vertex is at $$(2, 5)$$.

Next, let's find two more points to help us draw the parabola. We will pick $$x = 1$$ and $$x = 3$$, which are equally spaced around $$x = 2$$.

**For $$x = 1:$$**
- When $$x = 1$$, plug it into the equation:
$$y = -2 \cdot (1 - 2)^2 + 5$$
$$y = -2 \cdot 1^2 + 5$$
$$y = -2 + 5$$
$$y = 3$$
So, we get the point $$(1, 3)$$.

**For $$x = 3:$$**
- When $$x = 3$$, plug it into the equation:
$$y = -2 \cdot (3 - 2)^2 + 5$$
$$y = -2 \cdot 1^2 + 5$$
$$y = -2 + 5$$
$$y = 3$$
So, we get the point $$(3, 3)$$.

Now we have:
- $$(2, 5)$$ (the vertex),
- $$(1, 3)$$,
- $$(3, 3)$$.

Let's plot these points on the graph:
- $$(1, 3)$$
- $$(2, 5)$$
- $$(3, 3)$$

By connecting these points smoothly, we can see the shape of the parabola. It opens downwards because of the negative sign in front of the $$-2$$.

And that's it! We've successfully determined and graphed our parabola. Great job!