Hey there! Today, I'm excited to share a technique with you called **completing the square**. This method can help you solve any quadratic equation and it's actually the foundation for something called the quadratic formula. I'll prove the quadratic formula using this technique in the next video, but for now, let's get to know it better.

Let's start with the quadratic equation $$x^2 - 4x = 5$$. I left some space here on purpose. In our last video, we saw that things get easier if the left side of the equation is a perfect square. With completing the square, we're going to turn our quadratic equation into a perfect square by adding and subtracting numbers on both sides.

To get started, we want to make the left-hand side a perfect square. There needs to be a number here so that if we square it and then double it, we get -4. Trust me, it will get clearer with a few examples.

We want our equation to look like this: $$x^2 - 4x + \text{something} = (x - a)^2$$. We don’t know what $$a$$ is yet, but we know that if we square $$(x - a)$$ we get $$x^2 - 2ax + a^2$$. 

Now, we know $$2a$$ must equal -4, which means $$a$$ is -2. If $$a$$ is -2, then $$a^2$$ is 4. So, let's add 4 to both sides of our initial equation. Why to both sides? Because we want to keep the equation balanced.

Updating our equation:
$$x^2 - 4x + 4 = 5 + 4$$

This simplifies to:
$$x^2 - 4x + 4 = 9$$

Now the left-hand side is a perfect square, so we rewrite it as:
$$(x - 2)^2 = 9$$

Next, we take the square root of both sides:
$$x - 2 = \pm 3$$

Solving for $$x$$, we get:
$$x = 2 \pm 3$$

So, $$x$$ could be $$2 + 3 = 5$$ or $$2 - 3 = -1$$.

We’ve now found our solutions: $$x = 5$$ or $$x = -1$$. You could solve this without completing the square by factoring, but completing the square always works, even for harder problems.

For example, consider $$10x^2 - 30x - 8 = 0$$. First, we simplify by dividing everything by 2:
$$5x^2 - 15x - 4 = 0$$

Next, divide by 5 to make the leading coefficient 1:
$$x^2 - 3x - \frac{4}{5} = 0$$

Move the constant term to the other side:
$$x^2 - 3x = \frac{4}{5}$$

To make the left-hand side a perfect square, take half of -3 (which is $$-\frac{3}{2}$$) and square it to get $$\frac{9}{4}$$. Add $$\frac{9}{4}$$ to both sides:
$$x^2 - 3x + \frac{9}{4} = \frac{4}{5} + \frac{9}{4}$$

Find a common denominator and combine:
$$\frac{4}{5} = \frac{16}{20}$$
$$\frac{9}{4} = \frac{45}{20}$$
Thus,
$$\frac{16}{20} + \frac{45}{20} = \frac{61}{20}$$

So our equation becomes:
$$\left(x - \frac{3}{2}\right)^2 = \frac{61}{20}$$

Taking the square root of both sides:
$$x - \frac{3}{2} = \pm \sqrt{\frac{61}{20}}$$

Finally, solve for $$x$$:
$$x = \frac{3}{2} \pm \sqrt{\frac{61}{20}}$$

You probably wouldn't manage this with simple factoring! Completing the square saves the day.

Feel free to try this with different quadratics. Completing the square is a reliable method for solving them, no matter how tricky they seem.