Sure! Let's work through this together. We want to solve the equation $$2x^2 + 3 = 75$$. It looks like we can make this simpler by isolating $$x^2$$ because there is only one term with $$x$$ in it. 

Here's how we do it step by step:

First, write down the equation again: 
$$2x^2 + 3 = 75$$

We want to get $$x^2$$ by itself, so the first step is to get rid of the 3 by subtracting 3 from both sides of the equation:
$$2x^2 + 3 - 3 = 75 - 3$$

Now the equation is:
$$2x^2 = 72$$

Next, we need to divide both sides by 2 to isolate $$x^2$$:
$$\frac{2x^2}{2} = \frac{72}{2}$$

This simplifies to:
$$x^2 = 36$$

To solve for $$x$$, we take the square root of both sides. Remember that the square root can be both positive and negative:
$$x = \pm\sqrt{36}$$

So, we have:
$$x = \pm 6$$

This means $$x$$ can be either 6 or -6 because $$6^2 = 36$$ and $$(-6)^2 = 36$$. 

To check if both solutions work, we can substitute them back into the original equation:

For $$x = 6$$:
$$2(6^2) + 3 = 2(36) + 3 = 72 + 3 = 75$$

For $$x = -6$$:
$$2(-6^2) + 3 = 2(36) + 3 = 72 + 3 = 75$$

Both solutions work, so we have $$x = 6$$ and $$x = -6$$. Great job!