Hey there! Let's try solving a system of equations using substitution, so we won't get outsmarted by talking birds! Here's the problem we need to solve:

$$
-3x - 4y = -2
$$

and

$$
y = 2x - 5
$$

First, let's rewrite these equations clearly:

$$
-3x - 4y = -2
$$

and

$$
y = 2x - 5
$$

It's great that the second equation is already solved for $$y$$. This makes it easy to substitute. We'll take the expression for $$y$$ from the second equation and substitute it into the first equation.

So, the first equation becomes:

$$
-3x - 4(2x - 5) = -2
$$

Now, let's solve for $$x$$. We'll distribute the $$-4$$:

$$
-3x - 4(2x - 5) = -3x - 8x + 20 = -2
$$

Now, combine the $$x$$ terms:

$$
-3x - 8x = -11x
$$

So, the equation is now:

$$
-11x + 20 = -2
$$

To solve for $$x$$, we subtract 20 from both sides:

$$
-11x = -22
$$

Then, we divide both sides by $$-11$$:

$$
x = \frac{-22}{-11} = 2
$$

So, $$x = 2$$. But we're not done yet! We need to find $$y$$ too. We'll use the second equation:

$$
y = 2x - 5
$$

Since we know $$x = 2$$, substitute $$2$$ in place of $$x$$:

$$
y = 2(2) - 5 = 4 - 5 = -1
$$

So, $$y = -1$$. Let's check our solutions in the first equation to make sure they work:

If $$x = 2$$ and $$y = -1$$, then:

$$
-3(2) - 4(-1) = -6 + 4 = -2
$$

And it matches! So, the solutions are $$x = 2$$ and $$y = -1$$. You can now confidently type it in. Great job!

And there you have it, we won't be embarrassed by talking birds now!