Sure! Let's work through this together and make it as simple as possible.

### First Equation
We start with this equation:
$$a - x + 3x = b - x + 5$$

Let's solve for $$x$$ step-by-step.

1. **Group all the $$x$$ terms on the left-hand side.**
    - We have $$a - x + 3x$$ on the left.
    - We need to move $$b - x$$ from the right to the left by subtracting $$b - x$$ from both sides. This gives us:
    $$a - x + 3x - b + x = 5$$

2. **Simplify the left side.**
    - Combine like terms:
    $$a + 3x - b - x = 5$$

3. **Factor $$x$$ out.**
    - We rewrite the left side as:
    $$x \cdot (a - c - b + 3) = 5$$

4. **Solve for $$x$$.**
    - Now, divide both sides by $$a + 3 - b$$:
    $$x = \frac{5}{a + 3 - b}$$

And we're done with the first part!

### Second Equation
Now, let's look at the second equation:
$$a \cdot (5 - x) = b - x - 8$$

We will solve it step-by-step.

1. **Expand the left side by distributing $$a.$$**
    - That gives us:
    $$5a - ax = b - x - 8$$

2. **Move all $$x$$ terms to the left and non-$$x$$ terms to the right.**
    - Subtract $$b - x$$ from both sides, and subtract $$5a$$ from both sides:
    $$5a - ax - b + x = -8 - 5a$$

3. **Simplify the left side.**
    - Combine like terms:
    $$-ax + x - b = -8 - 5a$$

4. **Multiply both sides by -1 to get rid of negative signs.**
    - This gives us:
    $$ax - x + b = 8 + 5a$$

5. **Factor $$x$$ out.**
    $$x \cdot (a + 1) = 8 + 5a$$

6. **Solve for $$x$$.**
    - Finally, divide both sides by $$a + b$$:
    $$x = \frac{8 + 5a}{a + b}$$

And we have solved both equations for $$x$$! Nice work!