Sure, let's go through this step-by-step together.

First, we have a function $$g$$ that describes an arithmetic sequence. Here are the first few terms of this sequence:

- The first term is 4
- The second term is 3 4/5
- The third term is 3 3/5
- The fourth term is 3 2/5

We need to find the values of the missing parameters $$A$$ and $$B$$ in the recursive definition of the sequence given by:

$$g(n) = A \text{ if } n = 1$$
$$g(n) = g(n-1) + B \text{ if } n > 1$$

Let's start by identifying $$A$$. This part is pretty easy. When $$n = 1$$, we are given that the first term is 4. So, $$A = 4$$.

Next, we look at the second part of the definition, which uses the previous term to find the current term.

When we go from the first term (4) to the second term (3 4/5), we notice that we have subtracted $$1/5$$. This pattern continues for all subsequent terms:
- From 3 4/5 to 3 3/5, we also subtract $$1/5$$.
- From 3 3/5 to 3 2/5, again we subtract $$1/5$$.

So, every time we move from one term to the next, we are subtracting $$1/5$$. That means $$B = -1/5$$.

To restate:

- $$A = 4$$ because the first term is 4.
- $$B = -1/5$$ because we subtract $$1/5$$ each time to get the next term.

Now, we can complete our recursive definition:
$$g(n) = 4 \text{ if } n = 1$$
$$g(n) = g(n-1) - 1/5 \text{ if } n > 1$$

And there you have it! The values of $$A$$ and $$B$$ are 4 and $$ -1/5$$, respectively.