Sure, let's walk through this step-by-step to solve the quadratic equation using simple words so it feels like a friendly chat. We are asked to solve the equation:

$$ -3x^2 + 10x - 3 = 0 $$

This is already in the 'standard form' for quadratics. There are many ways to solve it, but we'll use the quadratic formula. Here’s how it looks:

$$ a = -3 $$
$$ b = 10 $$
$$ c = -3 $$

Remember, the quadratic formula is:

$$ x = \frac{-b \pm \sqrt{b^2 - 4ac}}{2a} $$

This formula helps us find the values of $$ x $$ that make our equation true. The $$ \pm $$ symbol means we will get two answers, one for "+" and one for "-".

Now, let’s plug in the values for $$ a $$, $$ b $$, and $$ c $$:

1. Start with $$ -b $$:
    $$ -b = -10 $$

2. Next, calculate $$ b^2 $$:
    $$ b^2 = 10^2 = 100 $$

3. Now, find $$ 4ac $$:
    $$ 4ac = 4 \times (-3) \times (-3) = 36 $$

4. Subtract $$ 4ac $$ from $$ b^2 $$:
    $$ b^2 - 4ac = 100 - 36 = 64 $$

5. Take the square root of 64:
    $$ \sqrt{64} = 8 $$

6. Finally, put it all together using the quadratic formula:
    $$ x = \frac{-10 \pm 8}{2 \times -3} $$

Now let's solve for both answers:

1. For the positive square root:
    $$ x = \frac{-10 + 8}{-6} = \frac{-2}{-6} = \frac{1}{3} $$

2. For the negative square root:
    $$ x = \frac{-10 - 8}{-6} = \frac{-18}{-6} = 3 $$

So, our solutions are $$ x = \frac{1}{3} $$ and $$ x = 3 $$.

But let’s do it again, in a different way by multiplying both sides of the equation by -1. Our equation becomes:

$$ 3x^2 - 10x + 3 = 0 $$

Here, $$ a = 3 $$, $$ b = -10 $$, and $$ c = 3 $$.

Using the quadratic formula again:

1. Start with $$ -b $$:
    $$ -b = 10 $$

2. Calculate $$ b^2 $$:
    $$ b^2 = (-10)^2 = 100 $$

3. Now, find $$ 4ac $$:
    $$ 4ac = 4 \times 3 \times 3 = 36 $$

4. Subtract $$ 4ac $$ from $$ b^2 $$:
    $$ b^2 - 4ac = 100 - 36 = 64 $$

5. Take the square root of 64:
    $$ \sqrt{64} = 8 $$

6. Finally, put it all together using the quadratic formula:
    $$ x = \frac{10 \pm 8}{2 \times 3} $$

Again we solve for both answers:

1. For the positive square root:
    $$ x = \frac{10 + 8}{6} = \frac{18}{6} = 3 $$

2. For the negative square root:
    $$ x = \frac{10 - 8}{6} = \frac{2}{6} = \frac{1}{3} $$

As a result, we get the same solutions: $$ x = 3 $$ and $$ x = \frac{1}{3} $$.

I hope this was clear and helpful! If you have any more questions, feel free to ask.