Hey there! Let's dive into some graph fun together! We have two types of functions: a linear one and an exponential one. They both go through the points (-1, 9) and (1, 1). Let's break this down step by step.

First, let’s look at the linear function \( f(x) = mx + b \). Using the points given, we need to find the slope, which is \( m \). The slope is calculated by the change in y over the change in x. For the points (1, 1) and (-1, 9):

- Change in x: \( 1 - (-1) = 2 \)
- Change in y: \( 1 - 9 = -8 \)

So, the slope \( m \) is:  
$$ m = \frac{{\text{{change in y}}}}{{\text{{change in x}}}} = \frac{-8}{2} = -4 $$

Now our equation looks like this:  
$$ f(x) = -4x + b $$

To find \( b \), use one of the points, let’s pick (1, 1):

- \( f(1) = -4 \cdot 1 + b = 1 \)
- \( -4 + b = 1 \)
- \( b = 5 \)

Therefore, our linear function is:  
$$ f(x) = -4x + 5 $$

Next, let's explore the exponential function \( g(x) = a \cdot r^x \). Given the points, we can set up two equations:

From the point (-1, 9):

- \( g(-1) = a \cdot r^{-1} = \frac{a}{r} = 9 \)
- \( a = 9r \)

From the point (1, 1):

- \( g(1) = a \cdot r = 1 \)
- \( a \cdot r = 1 \)

We now have two equations:

1. \( a = 9r \)
2. \( a \cdot r = 1 \)

Substitute \( a \) from the first equation into the second equation:

- \( 9r \cdot r = 1 \)
- \( 9r^2 = 1 \)
- \( r^2 = \frac{1}{9} \)
- \( r = \frac{1}{3} \) (since \( r > 0 \))

Finally, substitute \( r \) back into \( a = 9r \):

- \( a = 9 \cdot \frac{1}{3} = 3 \)

Therefore, our exponential function is:  
$$ g(x) = 3 \cdot \left(\frac{1}{3}\right)^x $$

There you go! We've found both functions. The linear function is \( f(x) = -4x + 5 \), and the exponential function is \( g(x) = 3 \cdot \left(\frac{1}{3}\right)^x \). Great job!