Sure, let's dive into recognizing the slope and y-intercept from different equations. I’ll guide you through it in a friendly, easy-to-understand way.

Let’s start with an equation you might recognize: $$y = 5x + 3$$. Here, we need to find the slope and the y-intercept. These terms come from the slope-intercept form of an equation, which is: $$y = mx + b$$. In this form, $$m$$ represents the slope, and $$b$$ is the y-intercept.

So, looking at $$y = 5x + 3$$:
- $$m = 5$$ (the number in front of $$x$$), making the slope $$5$$.
- $$b = 3$$ (the constant term), making the y-intercept $$3$$.

Let’s try another one: $$y = 5 + 3x$$. At first, this might look different, but remember, we're just adding terms, so their order doesn’t matter. We can rewrite it as $$y = 3x + 5$$. Now:
- $$m = 3$$, so the slope is $$3$$.
- $$b = 5$$, so the y-intercept is $$5$$.

Now, let’s look at: $$y = 12 - x$$. To match the slope-intercept form ($$y = mx + b$$), we can rewrite it as $$y = -x + 12$$. This means:
- The constant term (the y-intercept) is $$12$$, so $$b = 12$$.
- The slope is the coefficient in front of $$x$$, which we can write as $$-1x$$, so $$m = -1$$.

Next example: $$y = 5x$$. You might think it looks different because it only has one term on the right side. But we can think of it as $$y = 5x + 0$$. Now:
- $$m = 5$$, so the slope is $$5$$.
- $$b = 0$$, so the y-intercept is $$0$$.

For a final example: $$y = -7$$. This one also looks different, but we can write it as $$y = 0x - 7$$. So:
- $$m = 0$$, since there's no $$x$$ term, so the slope is $$0$$.
- $$b = -7$$, making the y-intercept $$-7$$.

Hope this helps!