Sure, let's go through this together:

We have a graph of the function $$f(x)$$, and we know it's an exponential function. It kind of looks like one, but it's always good to have confirmation. In this lesson, our goal is to find out at what value of $$x$$ the function $$f(x)$$ is equal to $$-\frac{1}{25}$$. You might think about guessing by looking at the graph, but that's tricky since $$-\frac{1}{25}$$ is just below the x-axis. Eyeballing it isnâ€™t exact, and we could make a mistake. So instead of guessing, let's find an expression for $$f(x)$$ using the information given, and then solve for $$x$$.

We know $$f(x)$$ is an exponential function, which generally looks like this: $$f(x) = a \cdot r^x$$. Here, $$a$$ is the initial value, or the value when $$x = 0$$. From the graph, we can see that when $$x = 0$$, $$f(0) = -25$$. So $$a = -25$$.

Next, we need to find the common ratio, $$r$$. This is the ratio between successive values of the function. The ratio could be between $$f(1)$$ and $$f(0)$$, or $$f(2)$$ and $$f(1)$$, and so on. We see from the graph that $$f(1) = -5$$. So the ratio is:

$$r = \frac{f(1)}{f(0)} = \frac{-5}{-25} = \frac{1}{5}$$

Now we can write our function:

$$f(x) = -25 \cdot \left(\frac{1}{5}\right)^x$$

Our next step is to find out when this function equals $$-\frac{1}{25}$$:

$$-25 \cdot \left(\frac{1}{5}\right)^x = -\frac{1}{25}$$

To solve for $$x$$, we should first divide both sides by $$-25$$:

$$\left(\frac{1}{5}\right)^x = \frac{1}{625}$$

We know that $$\left(\frac{1}{5}\right)^x$$ is the same as $$\frac{1}{5^x}$$, so:

$$\frac{1}{5^x} = \frac{1}{625}$$

This means $$5^x$$ must equal 625. We can now figure out what power of 5 gives us 625 by thinking about the powers of 5:

$$5^1 = 5$$
$$5^2 = 25$$
$$5^3 = 125$$
$$5^4 = 625$$

So, $$x = 4$$. 

Therefore, $$f(4) = -\frac{1}{25}$$.

You can check this by plugging in 4 back into the function to make sure it works. And there you go! Hopefully, this clears things up.