Hey there! Let's see if we can solve this equation together. We have:

$$ (2X - 3)^2 = 4X - 6 $$

I think you can try it yourself first, but I'll give you a little hint. You could do it the usual long way by expanding everything out and making it a classic quadratic equation. But there's a quicker and simpler way. Let's look closely at both sides of the equation.

On the left side, you have:

$$ (2X - 3)^2 $$

On the right side, you have:

$$ 4X - 6 $$

If you notice, $$ 4X - 6 $$ is just $$ 2 \times (2X - 3) $$, right? So we can write the equation like this:

$$ (2X - 3)^2 = 2 \times (2X - 3) $$

That's pretty interesting! We have something squared equal to two times that same thing. So, let's call this something $$ P $$. Let's say:

$$ P = 2X - 3 $$

Now, our equation becomes:

$$ P^2 = 2P $$

We just need to solve this for $$ P $$. Let's rearrange it:

$$ P^2 - 2P = 0 $$

We can factor out a $$ P $$:

$$ P(P - 2) = 0 $$

This tells us that either:

$$ P = 0 $$

or

$$ P - 2 = 0 $$, which means $$ P = 2 $$.

So, we have two possible values for $$ P $$: $$ 0 $$ or $$ 2 $$.

But remember, we need to find $$ X $$, not $$ P $$. So letâ€™s go back to our substitution:

$$ 2X - 3 = P $$

First case:

$$ 2X - 3 = 0 $$

Add 3 to both sides:

$$ 2X = 3 $$

Divide by 2:

$$ X = \frac{3}{2} $$

Second case:

$$ 2X - 3 = 2 $$

Add 3 to both sides:

$$ 2X = 5 $$

Divide by 2:

$$ X = \frac{5}{2} $$

So the possible solutions are:

$$ X = \frac{3}{2} $$ or $$ X = \frac{5}{2} $$.

Isn't that cool? By spotting the pattern, we avoided a lot of extra steps. If we had expanded and simplified everything in the usual way, it would have taken much longer. This method was quicker and simpler. Great job noticing the patterns in the equations!