Sure! Let's go through it together step by step.

We need to solve for $$s$$ and we have the equation:

$$s^2 - 2s - 35 = 0$$

This is a quadratic equation. While you might want to use regular algebra to solve it, the best way here is to factor the left side since it's equal to zero.

Let's factor it. To factor by grouping, find two numbers that add up to $$-2$$ and multiply to $$-35$$. Since the product is negative, one number will be positive, and the other will be negative. The numbers are 5 and -7, because:

$$5 + (-7) = -2$$ 

and

$$5 \times (-7) = -35$$

We can split the middle term like this:

$$s^2 + 5s - 7s - 35 = 0$$

Group them:

$$(s^2 + 5s) + (-7s - 35) = 0$$

Factor out the common parts:

$$s(s + 5) - 7(s + 5) = 0$$

Now, factor out $$(s + 5)$$:

$$(s + 5)(s - 7) = 0$$

We have a product of two numbers equal to zero. This means either:

$$s + 5 = 0$$ 

or

$$s - 7 = 0$$

Solve these simple equations:

$$s = -5$$

and

$$s = 7$$

So, $$s = -5$$ and $$s = 7$$ are our solutions. You can check them by plugging them back into the original equation:

For $$s = -5$$:

$$(-5)^2 - 2(-5) - 35 = 25 + 10 - 35 = 0$$

And for $$s = 7$$:

$$7^2 - 2 \times 7 - 35 = 49 - 14 - 35 = 0$$

Both work!

There's also a quicker way since the leading coefficient is 1. If we have something like $$(x + a)(x + b)$$, it expands to:

$$x^2 + (a+b)x + ab$$

Here, we want numbers that add to $$-2$$ and multiply to $$-35$$. We've found them: 5 and -7. 

So, we could have directly factored:

$$(s + 5)(s - 7)$$

This confirms our previous work and shows both methods are valid. Great job!