Sure, let's work on solving more systems of equations using elimination. But this time, it won't be just a one-step elimination. We’ll have to adjust the equations a bit before we can eliminate any variables.

Imagine we start with these two equations:

$$5x - 10y = 15$$
$$3x - 2y = 3$$

We want to solve these using elimination. While we could use substitution, or even graph these lines to find out where they intersect, we are focusing on elimination here.

The first step is recognizing that simply adding or subtracting these equations won't help right away because adding the left or right sides doesn’t eliminate any variables. Adding the left-hand sides would give us $$8x - 12y$$, which still has both $$x$$ and $$y$$ in it. So we need to make these equations look a bit different first.

We can multiply both equations in such a way that one of the terms cancels out. Let’s decide to cancel out the $$y$$ terms. Here’s a step-by-step for how we do it:

First, rewrite the original first equation just as it is:
$$5x - 10y = 15$$

Next, think about what we need to multiply the second equation by so that the $$y$$ terms will cancel each other out with the $$-10y$$ term in the first equation. If we multiply $$3x - 2y = 3$$ by $$-5$$, we can achieve this because $$-5 \times (-2y) = 10y$$. Let's do this:

Multiply the whole equation by $$-5$$:
$$-5 \times 3x = -15x$$
$$-5 \times (-2y) = 10y$$
$$-5 \times 3 = -15$$

This gives us the new equation:
$$-15x + 10y = -15$$

Now we’re ready to add this new equation to the first equation:
$$5x - 10y = 15$$
$$-15x + 10y = -15$$

Adding these together, the $$y$$ terms cancel out:
$$(5x - 15x) + (-10y + 10y) = 15 - 15$$
$$-10x = 0$$

Solving for $$x$$ by dividing by $$-10$$:
$$x = 0$$

With $$x = 0$$, substitute back into the original first equation to find $$y$$:
$$5 \times 0 - 10y = 15$$
$$-10y = 15$$

Divide both sides by $$-10$$:
$$y = -\frac{3}{2}$$

So, $$x = 0$$ and $$y = -\frac{3}{2}$$. The solution to the system is the point $$(0, -\frac{3}{2})$$. You can double-check this solution by plugging these values into the second equation to verify.

Now, let’s solve another system. Suppose we have:
$$5x + 7y = 15$$
$$7x - 3y = 5$$

Let’s eliminate the $$x$$ variables this time. To do that, we need to make the coefficients of $$x$$ the same or opposites. We can multiply the first equation by $$7$$ and the second by $$-5$$ so that their $$x$$ terms become opposites and cancel out when added:

Multiply the first equation:
$$7 \times (5x + 7y) = 7 \times 15$$
$$35x + 49y = 105$$

Multiply the second equation:
$$-5 \times (7x - 3y) = -5 \times 5$$
$$-35x + 15y = -25$$

Now add these two new equations:
$$35x + 49y$$
$$-35x + 15y$$
\(-----\)
$$64y = 80$$

Solving for $$y$$:
$$y = \frac{80}{64} = \frac{5}{4}$$

Substitute $$y = \frac{5}{4}$$ back into one of the original equations to find $$x$$. Let’s choose the second equation:
$$7x - 3 \left(\frac{5}{4}\right) = 5$$
$$7x - \frac{15}{4} = 5$$

Add $$\frac{15}{4}$$ to both sides:
$$7x = 5 + \frac{15}{4}$$
$$7x = \frac{20}{4} + \frac{15}{4} = \frac{35}{4}$$

Solve for $$x$$ by dividing by $$7$$:
$$x = \frac{35}{4} \times \frac{1}{7} = \frac{5}{4}$$

So, the solution is $$(\frac{5}{4}, \frac{5}{4})$$. Double-check by plugging these values into the original equations, and we see they satisfy both equations.

That's how you solve systems of equations using elimination. It might look complicated at first, but with practice, it becomes much easier!