Sure! Let's break it down step by step together. Here’s the process presented in an easier way:

1. We start with the function $$f(x) = -x + 4$$.
   
2. The function $$f(x)$$ is already graphed on our coordinate plane.

3. To find the inverse, we set it up as $$y = f(x)$$. So, we have:
   $$y = -x + 4$$

4. Now let's solve for $$x$$ in terms of $$y$$. First, subtract 4 from both sides:
   $$y - 4 = -x$$

5. Then multiply both sides by $$-1$$ to solve for $$x$$:
   $$-y + 4 = x$$

6. We can rewrite it to make it look more familiar:
   $$x = -y + 4$$

7. So, the inverse function $$f^{-1}(y)$$ is:
   $$f^{-1}(y) = -y + 4$$

8. But, since we usually write functions using $$x$$, we rename $$y$$ as $$x$$:
   $$f^{-1}(x) = -x + 4$$

9. Interestingly, the inverse is the same as the original function. We can check that they are reflections over the line $$y = x$$.

10. Now, let's think about another example. Let's start with $$g(x) = -2x - 1$$.

11. We'll set it as $$y = g(x)$$, so:
    $$y = -2x - 1$$

12. Next, solve for $$x$$. First, add 1 to both sides:
    $$y + 1 = -2x$$

13. Then divide by $$-2$$:
    $$\frac{y + 1}{-2} = x$$

14. Simplify it:
    $$x = -\frac{y}{2} - \frac{1}{2}$$

15. So the inverse $$g^{-1}(y)$$ is:
    $$g^{-1}(y) = -\frac{y}{2} - \frac{1}{2}$$

16. We rename $$y$$ as $$x$$, so:
   $$g^{-1}(x) = -\frac{x}{2} - \frac{1}{2}$$

17. We can graph this inverse function to see it reflected over $$y = x$$. Start at the y-intercept, $$-1/2$$. 

18. With a slope of $$-1/2$$, you’ll see the line moves like described. 

19. When graphed, you can notice that it indeed reflects over the line $$y = x$$. 

So basically, finding the inverse function involves switching $$x$$ and $$y$$, solving for $$x$$, and then renaming to put it back in function terms. And graphing helps us see how the original and the inverse are related. Isn't that cool? Let me know if you have any questions!