Hey there! Let’s take a look at this table where we have some values for $$n$$ and $$f(n)$$. When $$n = 1$$, $$f(1) = 12$$; when $$n = 2$$, $$f(2) = 5$$; when $$n = 3$$, $$f(3) = -2$$; and when $$n = 4$$, $$f(4) = -9$$. 

This function $$f$$ is creating a sequence:
- First term: 12
- Second term: 5
- Third term: -2
- Fourth term: -9

And it continues like this.

You might notice that it looks like an arithmetic sequence. We start with 12 and then subtract 7 to get to the next term (12 - 7 = 5). To move from the second to the third term, we subtract 7 again (5 - 7 = -2). Each term is 7 less than the one before it.

Now, can we define this function $$f(n)$$ more clearly? We want to find a formula for $$f(n)$$. Here’s how we can think about it:

We start with 12 for the first term. For the second term, we subtract 7 just once:
- For the third term, we subtract 7 twice.
- For the fourth term, we subtract 7 three times.

So, for any term $$n$$, we subtract 7 $$(n - 1)$$ times.

Let's put this into a formula:
$$ f(n) = 12 - 7 \times (n - 1) $$

We can check if this works:
- For $$f(1)$$, $$n = 1$$: $$ 12 - 7 \times (1 - 1) = 12 - 0 = 12 $$
- For $$f(2)$$, $$n = 2$$: $$ 12 - 7 \times (2 - 1) = 12 - 7 = 5 $$
- For $$f(3)$$, $$n = 3$$: $$ 12 - 7 \times (3 - 1) = 12 - 14 = -2 $$

It works!

Now, let’s do another example. Look at this sequence from the table:
- First term: -100
- Second term: -50
- Third term: 0
- Fourth term: 50

Here, we start at -100 and add 50 each time. This is also an arithmetic sequence. Each term is 50 more than the one before.

Let’s define the function $$f(n)$$ for this sequence. One way to think about it:
Starting at -100, we add 50 $$(n - 1)$$ times.

So, the formula is:
$$ f(n) = -100 + 50 \times (n - 1) $$

We can check if this formula works:
- For $$f(1)$$, $$n = 1$$: $$ -100 + 50 \times (1 - 1) = -100 + 0 = -100 $$
- For $$f(2)$$, $$n = 2$$: $$ -100 + 50 \times (2 - 1) = -100 + 50 = -50 $$
- For $$f(3)$$, $$n = 3$$: $$ -100 + 50 \times (3 - 1) = -100 + 100 = 0 $$

This checks out!

There are other ways to write this function too. Another formula could be:
$$ f(n) = -150 + 50n $$

To see if it works, we check:
- For $$f(1)$$, $$n = 1$$: $$ -150 + 50 \times 1 = -150 + 50 = -100 $$
- For $$f(2)$$, $$n = 2$$: $$ -150 + 50 \times 2 = -150 + 100 = -50 $$
- For $$f(3)$$, $$n = 3$$: $$ -150 + 50 \times 3 = -150 + 150 = 0 $$

This one works too!

Why do these two formulas work even though they look different? Because we can rewrite the first one as:
$$ -100 + 50(n - 1) $$
Distributing the 50, we get:
$$ -100 + 50n - 50 = -150 + 50n $$

So, the formulas $$ -100 + 50(n - 1) $$ and $$ -150 + 50n $$ are actually the same!

But the formula:
$$ -100 + 50n $$
Doesn’t work because when $$ n = 1 $$, it gives us:
$$ -100 + 50 = -50 $$ 

Instead of -100.

And that’s it! We’ve defined $$f(n)$$ for these sequences and even checked our work. Nice job!