Hey there! Let's work on solving this quadratic equation together: $$x^2 - 2x - 8 = 0$$. By the way, sorry if you hear some noise; they're cutting trees outside, but let's focus on the problem!

There are a few ways to solve this, but we'll use a method called "completing the square." This means we'll rewrite the equation to look like $$ (x + a)^2 + b $$, and then solve it easily from there.

First, let's see how we expand $$ (x + a)^2 $$. If we expand it, we get:

$$ (x + a)^2 = x^2 + 2ax + a^2 $$

Now, let's go back to our original equation and add some space so we can work with it:

$$ x^2 - 2x - 8 = 0 $$

We'll rewrite it as:

$$ x^2 - 2x \quad\textcolor{gray}{\_} - 8 \quad\textcolor{gray}{\_} = 0 $$

Next, we'll match our equation to the expanded form we discussed. For $$ x^2 - 2x $$ to match $$ x^2 + 2ax $$, we see that $$ 2a = -2 $$, which means $$ a = -1 $$.

Now, we need to add $$ a^2 $$, which is $$ (-1)^2 = 1 $$:

$$ x^2 - 2x + 1 - 1 - 8 = 0 $$

Adding 1 and then subtracting it keeps the equation the same. Let's group the completed square:

$$ (x - 1)^2 - 9 = 0 $$

To solve this, we'll add 9 to both sides:

$$ (x - 1)^2 = 9 $$

Now, we take the square root of both sides, remembering it can be positive or negative:

$$ x - 1 = \pm 3 $$

So we have two solutions:

1. $$ x - 1 = 3 \rightarrow x = 4 $$
2. $$ x - 1 = -3 \rightarrow x = -2 $$

Therefore, the solutions are:

$$ x = 4 \quad\text{or}\quad x = -2 $$

Some might wonder why we used completing the square. While we could have factored it directly, completing the square is handy because it works for all quadratic equations. You'll also find it useful when learning about the quadratic formula in the future!

Hope you enjoyed that!