Sure! Let's chat about how to solve this problem step-by-step.

We need to solve the equation $$-x^2 + 8x = 1$$ using the quadratic formula. But first, we should rewrite the equation in the standard form $$ax^2 + bx + c = 0$$.

To do this, let's subtract 1 from both sides:
$$-x^2 + 8x - 1 = 0$$

Now it looks like $$ax^2 + bx + c = 0$$, where:
- $$a = -1$$
- $$b = 8$$
- $$c = -1$$

The quadratic formula is:
$$x = \frac{-b \pm \sqrt{b^2 - 4ac}}{2a}$$

We can now plug in our values for $$a$$, $$b$$, and $$c$$:
$$x = \frac{-8 \pm \sqrt{8^2 - 4(-1)(-1)}}{2(-1)}$$

Let's simplify what's inside the square root first:
$$8^2 = 64$$
$$-4 \cdot (-1) \cdot (-1) = 4$$

So we have:
$$x = \frac{-8 \pm \sqrt{64 - 4}}{2(-1)}$$
$$x = \frac{-8 \pm \sqrt{60}}{-2}$$

Next, we simplify the square root of 60. We know that:
$$\sqrt{60} = \sqrt{4 \cdot 15} = \sqrt{4} \cdot \sqrt{15} = 2\sqrt{15}$$

Now we can rewrite the formula:
$$x = \frac{-8 \pm 2\sqrt{15}}{-2}$$

We can separate this into two parts:
$$x = \frac{-8}{-2} \pm \frac{2\sqrt{15}}{-2}$$

Simplifying each part, we get:
$$x = 4 \mp \sqrt{15}$$

So, the solutions to the equation are:
$$x = 4 - \sqrt{15} \quad \text{and} \quad x = 4 + \sqrt{15}$$

Both of these values for $$x$$ will satisfy the original equation. If anything is confusing, just let me know. I'm here to help you understand!