Sure, let's work through this together! Here’s how we can solve for $$x$$ in different situations:

### Solving the Equation:

First, we're going to solve an equation. Let's say we have an equation that looks like this:

$$x + 3$$ squared $$- 4 = 0$$

We need to find the $$x$$ values that make this equation true. Here’s a step-by-step process:

1. Add 4 to both sides to get rid of the $$-4$$.
    - This leaves us with:
      $$(x + 3)^2 = 4$$
      
2. Take the square root of both sides. Remember that the square root of 4 can be either 2 or -2.
    - So, we have:
      $$x + 3 = \pm 2$$
      
3. Split the solution into two cases:
    - $$x + 3 = 2$$
    - $$x + 3 = -2$$
    
4. Solve each case separately by subtracting 3 from both sides.
    - For $$x + 3 = 2$$:
      $$x = 2 - 3 = -1$$
      
    - For $$x + 3 = -2$$:
      $$x = -2 - 3 = -5$$
      
So, the solutions for the equation are $$x = -1$$ and $$x = -5$$.

### Verifying Our Solutions:

To check if our solutions are correct, we can substitute $$x = -1$$ and $$x = -5$$ back into the original equation:

- For $$x = -1$$:
  - $$(-1 + 3)^2 - 4 = (2)^2 - 4 = 4 - 4 = 0$$ (True)
  
- For $$x = -5$$:
  - $$(-5 + 3)^2 - 4 = (-2)^2 - 4 = 4 - 4 = 0$$ (True)

### Finding Intersection Points on a Graph:

Next, let’s find where the graph of a function $$y = f(x)$$ intersects the x-axis. For this, let’s start with:

$$f(x) = (x - 2)^2 - 9$$

To find where this function intersects the x-axis, we need to find the $$x$$ values where $$f(x) = 0$$.

1. Set $$f(x)$$ to 0:
    - $$(x - 2)^2 - 9 = 0$$
    
2. Add 9 to both sides:
    - $$(x - 2)^2 = 9$$
    
3. Take the square root of both sides, remembering it can be either positive or negative:
    - $$x - 2 = \pm 3$$
    
4. Solve each case by adding 2 to both sides:
    - For $$x - 2 = 3$$:
      - $$x = 3 + 2 = 5$$
      
    - For $$x - 2 = -3$$:
      - $$x = -3 + 2 = -1$$
      
So, the $$x$$ values where the function intersects the x-axis are $$x = 5$$ and $$x = -1$$.

### Checking Points on the Graph:

To make sure, we substitute $$x = 5$$ and $$x = -1$$ back into the function:

- For $$x = 5$$:
  - $$(5 - 2)^2 - 9 = 3^2 - 9 = 9 - 9 = 0$$ (True)
  
- For $$x = -1$$:
  - $$(-1 - 2)^2 - 9 = (-3)^2 - 9 = 9 - 9 = 0$$ (True)

By working through these steps, we've not only solved for $$x$$, but also learned how to verify our solutions! Great job!