Alright, let's dive into this together! We're going to think of the function $$G$$ as a stretched and flipped version of the function $$F(x) = x^2$$. Here's how we can write the equation for $$G(x)$$. 

First, let's flip $$F(x)$$ over the x-axis. If we do this, our equation changes from $$y = x^2$$ to $$y = -x^2$$. Here’s why: 

1. When $$x = 0$$, $$y$$ stays $$0$$.
2. When $$x = 1$$, instead of $$y = 1$$, it becomes $$y = -1$$. 
3. When $$x = 2$$, instead of $$y = 4$$, it becomes $$y = -4$$.

Flipping it gives us $$y = -x^2$$. 

Next, we need to stretch this function horizontally and not just flip it. We do this stretching using a scaling factor. We pick a point that sits on $$G(x)$$, like $$2, -1$$. This point tells us that when $$x = 2$$, $$G(x) = -1$$.

For the flipped function $$y = -x^2$$, when $$x = 2$$, $$y = -4$$. To match this to $$G(x)$$, we need to multiply $$-4$$ by a fraction that gives us $$-1$$. That fraction is $$\frac{-1}{4}$$. So now, our equation becomes:

$$y = -\frac{1}{4}x^2$$.

Let’s check if this works:

1. When $$x = 1$$, $$1^2 = 1$$, and multiplying by $$-\frac{1}{4}$$ gives us $$-\frac{1}{4}$$.
2. When $$x = 2$$, $$2^2 = 4$$, and multiplying by $$-\frac{1}{4}$$ gives us $$-1$$.
3. When $$x = 4$$, $$4^2 = 16$$, and multiplying by $$-\frac{1}{4}$$ gives us $$-4$$.

This scaling factor works for both positive and negative values of $$x$$. So, we now know that the equation for $$G(x)$$ is $$ \boxed{G(x) = -\frac{1}{4}x^2}$$.

Just remember, flipping the function makes the output (or y-values) negative, which is why we multiply by -1. Stretching it horizontally involves a fraction smaller than 1, which makes the graph wider. 

And that's it! We've figured out the equation for $$G(x)$$! Great job!