Hey there! In this chat, we'll go through lots of examples of factoring second-degree polynomials, also known as quadratics. These are equations where the highest exponent of the variable is 2. For all our examples, we'll use the variable $$x$$.

Let's start with the quadratic expression $$x^2 + 10x + 9$$ and see how we can factor it into the product of two binomials. To do this, let's think about multiplying $$(x + a)$$ and $$(x + b)$$. If we multiply these, we get:

$$x \cdot x + x \cdot b + a \cdot x + a \cdot b = x^2 + (a + b)x + ab$$

Here, the middle term's coefficient (10 in this example) is the sum of $$a$$ and $$b$$, and the constant term (9) is the product of $$a$$ and $$b$$. So, we need to find numbers $$a$$ and $$b$$ such that:

$$a + b = 10$$ and $$a \cdot b = 9$$

Let's think about the factors of 9: 1, 3, and 9. If $$a$$ and $$b$$ are 1 and 9, then:

$$1 + 9 = 10$$ and $$1 \cdot 9 = 9$$

So, this works! We can factor the expression as $$(x + 1)(x + 9)$$. You can multiply them out to check that it matches $$x^2 + 10x + 9$$.

Let's try another one: $$x^2 + 15x + 50$$. We need $$a$$ and $$b$$ to satisfy:

$$a + b = 15$$ and $$a \cdot b = 50$$

Looking at factors of 50, we get combinations like 1 and 50, 2 and 25, and 5 and 10. Here, 5 and 10 work because:

$$5 + 10 = 15$$ and $$5 \cdot 10 = 50$$

So we can factor it as $$(x + 5)(x + 10)$$.

Let's make it a bit tricky with negative signs: $$x^2 - 11x + 24$$. We need:

$$a + b = -11$$ and $$a \cdot b = 24$$

Since the product is positive and the sum is negative, both numbers must be negative. Factors of 24 include 3 and 8, so considering negative values, we get $$-3$$ and $$-8$$:

$$-3 \cdot -8 = 24$$ and $$-3 + (-8) = -11$$

So, the factorization is $$(x - 3)(x - 8)$$.

How about mixing up positive and negative terms? Consider $$x^2 + 5x - 14$$. Here, we need:

$$a + b = 5$$ and $$a \cdot b = -14$$

The product is negative, so one must be positive and the other negative. Trying 2 and 7:

$$-2 + 7 = 5$$ and $$-2 \cdot 7 = -14$$

So, we factor it as $$(x - 2)(x + 7)$$.

Now, let's factor with a negative leading term: $$-x^2 - 5x + 24$$. First, factor out the negative:

$$-1(x^2 + 5x - 24)$$

Now, find $$a$$ and $$b$$ for the positive quadratic:

$$a + b = 5$$ and $$a \cdot b = -24$$

Trying factors of 24 like 3 and 8:

$$-3 + 8 = 5$$ and $$-3 \cdot 8 = -24$$

So the factorization is $$-1(x - 3)(x + 8)$$.

Finally, another example: $$-x^2 + 18x - 72$$. Factor out the negative:

$$-1(x^2 - 18x + 72)$$

Find $$a$$ and $$b$$ for:

$$a + b = -18$$ and $$a \cdot b = 72$$

Trying 6 and 12:

$$-6 + (-12) = -18$$ and $$-6 \cdot -12 = 72$$

So the factorization is $$-1(x - 6)(x - 12)$$.

Practicing these a few times will make this process a lot easier. Just remember to look at the coefficient sums for the middle term and the product for the constant term. Happy factoring!