Sure! Let's break it down step by step in a friendly and simple way:

You want to find the average rate of change of $$y$$ with respect to $$x$$ over the interval from $$x = -5$$ to $$x = -2$$. 

First, when $$x = -5$$, $$y$$ is equal to 6. And when $$x = -2$$, $$y$$ is equal to 0. 

To figure out the average rate of change of $$y$$ with respect to $$x$$, we need to look at how much $$y$$ changes divided by how much $$x$$ changes over this interval.

The symbol for change is a triangle, called "delta" (Î”). So, the change in $$y$$ is written as $$\Delta y$$ and the change in $$x$$ is written as $$\Delta x$$.

The average rate of change is then:
$$ \text{Average Rate of Change} = \frac{\Delta y}{\Delta x} $$

Let's find these changes:
- The change in $$y$$: $$\Delta y = 0 - 6 = -6$$ (since $$y$$ goes from 6 to 0, it decreases by 6).
- The change in $$x$$: $$\Delta x = -2 - (-5) = -2 + 5 = 3$$ (since $$x$$ goes from -5 to -2, it increases by 3).

Now, we put these values into the formula:

$$ \frac{-6}{3} = -2 $$

So, the average rate of change of $$y$$ with respect to $$x$$ over the interval from $$x = -5$$ to $$x = -2$$ is $$-2$$. This means that for every 1 unit increase in $$x$$, $$y$$ decreases by 2 units on average.