Sure! Let's go through this step by step together. I'll keep things simple and friendly:

---

Imagine we have an exponential function, which we'll call $$h(n)$$. Since it's an exponential function, it will look like this: $$h(n) = a \cdot r^n$$, where:
- $$a$$ is the starting value (initial value).
- $$r$$ is the common ratio (how much we multiply by each time).

We're assuming $$r$$ is greater than zero. We're given some information about $$h(n)$$:
- When $$n = 2$$, $$h(2) = 144$$
- When $$n = 4$$, $$h(4) = 324$$
- When $$n = 6$$, $$h(6) = 729$$

Using this information, we're going to find out what $$a$$ and $$r$$ are. 

First, let's focus on finding $$r$$. The common ratio $$r$$ tells us how the function grows. We could find $$r$$ between two successive values like $$h(3)$$ and $$h(2)$$, but we don't have $$h(3)$$. Instead, we can look at the ratio between $$h(4)$$ and $$h(2)$$:

$$\frac{h(4)}{h(2)} = \frac{324}{144}$$

Let's simplify $$\frac{324}{144}$$:
- Divide both by 2: $$\frac{162}{72}$$
- Divide by 2 again: $$\frac{81}{36}$$
- Divide by 9: $$\frac{9}{4}$$

So, the ratio is $$\frac{9}{4}$$. Using the exponential function form, we can rewrite:

$$\frac{h(4)}{h(2)} = \frac{a \cdot r^4}{a \cdot r^2} = r^{4-2} = r^2$$

Now we know:

$$r^2 = \frac{9}{4}$$

Since $$r$$ is greater than zero:

$$r = \sqrt{\frac{9}{4}} = \frac{3}{2}$$

Great, we've found $$r$$! Now, let's find $$a$$. One way to do this is to think about $$a$$ as the value of $$h(0)$$. We can use a table to understand this better, where each previous term is divided by the common ratio:

$$
\begin{array}{c|c}
n & h(n) \\
\hline
0 & a \\
1 & ? \\
2 & 144 \\
4 & 324 \\
6 & 729 \\
\end{array}
$$

We know $$r = \frac{3}{2}$$, so each step back divides by $$\frac{3}{2}$$:

- $$h(1) = \frac{144}{\frac{3}{2}} = 144 \cdot \frac{2}{3} = 96$$
- $$h(0) = \frac{96}{\frac{3}{2}} = 96 \cdot \frac{2}{3} = 64$$

So, $$a = 64$$.

Finally, we have the full function:

$$h(n) = 64 \cdot \left(\frac{3}{2}\right)^n$$

Another way to solve for $$a$$ is using one of the given points. Since we know $$r$$, we use $$h(2) = 144$$:

$$144 = a \cdot \left(\frac{3}{2}\right)^2 = a \cdot \frac{9}{4}$$

Solving for $$a$$:

$$a = 144 \cdot \frac{4}{9} = 64$$

So $$a = 64$$, confirming our function:

$$h(n) = 64 \cdot \left(\frac{3}{2}\right)^n$$

---

I hope you enjoyed working through this! Understanding how to break it down step-by-step makes it much easier to grasp. Keep practicing and you'll be a math whiz in no time!