Sure! Let's walk through this problem together to find the value of $$c$$ that makes $$x^2 - 44x + c$$ a perfect square trinomial, and then write it as the square of a binomial. A trinomial is just a polynomial with three terms.

To make $$x^2 - 44x + c$$ into a perfect square, we can look at the pattern for a perfect square trinomial. Let's think of it as $$(x + a)^2$$. This is the same as $$(x + a)(x + a)$$.

When we multiply this out, we get:
$$x \times x = x^2$$
$$x \times a = ax$$
$$a \times x = ax$$
$$a \times a = a^2$$

So, $$(x + a)^2 = x^2 + 2ax + a^2$$. If we compare this with $$x^2 - 44x + c$$, we can see that $$2a$$ must be equal to $$-44$$.

From $$2a = -44$$, we can solve for $$a$$ by dividing both sides by 2:
$$a = \frac{-44}{2} = -22$$.

Now we know $$a$$, we need to find $$c$$. Since $$c = a^2$$, we get:
$$c = (-22)^2 = 484$$.

So, if we rewrite $$x^2 - 44x + c$$ with $$c = 484$$, we get:
$$x^2 - 44x + 484$$. 

Now, if we want to write this as the square of a binomial, we notice that it's the same as:
$$x^2 - 2 \times 22x + 22^2$$, which is:
$$(x - 22)^2$$.

So, the original expression $$x^2 - 44x + c$$ can be written as:
$$x^2 - 44x + 484$$, which is:
$$(x - 22)^2$$.

I hope this makes sense! Let me know if you have any questions.