Sure thing! Let's go through this problem step by step, just like we are chatting and solving it together. Here's the equation: $$3 \times (x + 6)^2 = 75$$. First, let's see what steps we need to take to find the value of $$x$$.

1. **Divide Both Sides by 3**:
   To get rid of the $$3$$, we need to divide both sides of the equation by $$3$$. This gives us:
   $$\frac{3 \times (x + 6)^2}{3} = \frac{75}{3}$$.
   
   So, we are left with:
   $$(x + 6)^2 = 25$$.

2. **Take the Square Root of Both Sides**:
   Next, we need to eliminate the square. To do this, we take the square root of both sides. Remember, when you take the square root, you have to consider both the positive and negative roots:
   $$\sqrt{(x + 6)^2} = \pm \sqrt{25}$$.
   
   This simplifies to:
   $$x + 6 = \pm 5$$.

3. **Subtract 6 from Both Sides**:
   To isolate $$x$$, we need to get rid of the $$6$$ by subtracting $$6$$ from both sides:
   $$x + 6 - 6 = \pm 5 - 6$$,
   
   which simplifies to:
   $$x = -6 \pm 5$$.

So, we have two possible values for $$x$$:
- $$x = -6 + 5 = -1$$
- $$x = -6 - 5 = -11$$

And that's it! The steps we took were:
1. Divide both sides by 3.
2. Take the square root of both sides.
3. Subtract 6 from both sides.

This process gives us the solutions $$x = -1$$ or $$x = -11$$. Great job working through this with me!