Sure! Let's chat about it in a friendlier and simpler way:

Hey! So, we have this function called $$g$$, and it's an exponential one. It starts with a value of -2. This starting point is what we call the "initial value." Also, every time we move forward, we multiply by 1/7. This "1/7" is called the "common ratio."

Now, to write the formula for $$g(t)$$, we'll use a general form for exponential functions. It looks like this: 

$$g(t) = A \cdot r^t$$

Here, $$A$$ is the initial value and $$r$$ is the common ratio. From what we have, the initial value $$A$$ is -2, and the common ratio $$r$$ is 1/7. So, we put these values into the formula:

$$g(t) = -2 \cdot \left( \frac{1}{7} \right)^t$$

Letâ€™s make sense of this: if $$t$$ is 0, then 

$$\left( \frac{1}{7} \right)^0 = 1$$

This means 

$$g(0) = -2 \cdot 1 = -2$$

So, at $$t = 0$$, the function value is our initial value, -2. 

Now, every time $$t$$ goes up by 1, you multiply by 1/7 again. For instance, when $$t$$ is 1,

$$g(1) = -2 \cdot \left( \frac{1}{7} \right) = -\frac{2}{7}$$

When $$t$$ is 2,

$$g(2) = -2 \cdot \left( \frac{1}{7} \right)^2 = -2 \cdot \frac{1}{49} = -\frac{2}{49}$$

And so on. Each step, you just keep multiplying by 1/7, which is why we call it the "common ratio." I hope this helps and makes the concept clear for you!