Sure, I'd be happy to help with this! Let's break it down together.

We have a function \( g(x) \) that is equal to \( 9 \times 8^{x-1} \). This function is only defined for \( x \) being a positive whole number (like 1, 2, 3, etc.).

So, if we talk about the domain (all the valid inputs) for this function, it will be all the positive whole numbers: 1, 2, 3, 4, and so on. This means the function is defined directly.

Now, let’s try to write this same function using a recursive definition. A recursive definition tells us how to find the value at any \( x \) using the value at the previous \( x \).

First, let’s understand what happens when we put different values of \( x \) into the function. We'll make a table to see the pattern.

For \( x = 1 \), 
\[ g(1) = 9 \times 8^{1-1} = 9 \times 8^0 = 9 \times 1 = 9 \]

For \( x = 2 \), 
\[ g(2) = 9 \times 8^{2-1} = 9 \times 8^1 = 9 \times 8 \]

For \( x = 3 \), 
\[ g(3) = 9 \times 8^{3-1} = 9 \times 8^2 = 9 \times 8 \times 8 \]

For \( x = 4 \),
\[ g(4) = 9 \times 8^{4-1} = 9 \times 8^3 = 9 \times 8 \times 8 \times 8 \]

Notice the pattern? Starting from \( x = 2 \), each value is 8 times the previous value.

So, we can define the function recursively like this:

1. The base case, where \( x = 1 \), \( g(1) = 9 \).
2. For any \( x > 1 \), \( g(x) = g(x-1) \times 8 \).

Let’s verify this recursive definition to make sure it works.

When \( x = 1 \),
\[ g(1) = 9 \]

When \( x = 2 \),
\[ g(2) = g(1) \times 8 = 9 \times 8 \]

When \( x = 3 \),
\[ g(3) = g(2) \times 8 = (9 \times 8) \times 8 = 9 \times 8 \times 8 \]

When \( x = 4 \),
\[ g(4) = g(3) \times 8 = (9 \times 8 \times 8) \times 8 = 9 \times 8 \times 8 \times 8 \]

As you see, the recursive definition produces the same results as the original function. So, writing it recursively gives us:

\[ g(x) = 9 \text{ if } x = 1 \]
\[ g(x) = g(x-1) \times 8 \text{ if } x > 1 \]

This way, we have shown how you can express the function \( g(x) \) both directly and using a recursive approach!