Sure! Let's go through this step-by-step together. I'll break everything down plainly and use simple words. Here we go:

We have a line that goes through the points (-3, 6) and (6, 0). We need to find the equation of this line in three forms: point-slope form, slope-intercept form, and standard form. These are just different ways to write the same thing. If we write one form, we can change it to the others.

**First, let's understand these forms:**

- **Point-slope form:** If you know a point $$(x_1, y_1)$$ on the line and the slope $$(m)$$, then the equation is:

$$y - y_1 = m(x - x_1)$$

- **Slope-intercept form:** This is written as:

$$y = mx + b$$

Here, $$m$$ is the slope and $$b$$ is where the line meets the y-axis.

- **Standard form:** This is written as:

$$Ax + By = C$$

Here, $$A$$, $$B$$, and $$C$$ are numbers.

**Step 1: Find the Slope**

The slope $$m$$ is the change in y divided by the change in x. Using the points $$(x_1, y_1) = (-3, 6)$$ and $$(x_2, y_2) = (6, 0)$$,:

$$m = \frac{y_2 - y_1}{x_2 - x_1}$$

So,

$$m = \frac{0 - 6}{6 - (-3)} = \frac{-6}{9} = -\frac{2}{3}$$

**Step 2: Point-Slope Form**

Using the point $$(x_1, y_1) = (-3, 6)$$ and the slope $$m = -\frac{2}{3}$$:

$$y - 6 = -\frac{2}{3}(x + 3)$$

Simplifying it:

$$y - 6 = -\frac{2}{3}x - 2$$

**Step 3: Slope-Intercept Form**

We take the equation from the point-slope form and solve for $$y$$:

$$y - 6 = -\frac{2}{3}x - 2$$

Add 6 to both sides:

$$y = -\frac{2}{3}x + 4$$

So, $$y = -\frac{2}{3}x + 4$$ is our slope-intercept form.

**Step 4: Standard Form**

We want the x and y terms on one side:

$$- \frac{2}{3}x + y = 4$$

To get rid of the fraction, multiply everything by 3:

$$-2x + 3y = 12$$

So, our standard form is:

$$2x - 3y = -12$$

And there you have it! We've written the same line in point-slope form, slope-intercept form, and standard form. If you have any questions, feel free to ask!