Hey there! Let's chat about a fun topic today: exponential growth and exponential decay. We'll start with reviewing exponential growth. Imagine we have a table to help us out:

| x | y |
|---|---|
| 0 | 3 |
| 1 | 6 |
| 2 | 12 |
| -1 | 1.5 |

Now, let's say when $$ x = 0 $$, $$ y = 3 $$. Each time we increase $$ x $$ by 1, we double $$ y $$. So:

- When $$ x = 1 $$, $$ y $$ goes from 3 to 6.
- When $$ x = 2 $$, $$ y $$ becomes 12.

This doubling pattern shows us exponential growth. We can even go into negative $$ x $$ values:

- When $$ x = -1 $$, $$ y $$ is $$ \frac{3}{2} $$ or 1.5.

If we look at this with an equation, it would be: $$ y = 3 \cdot 2^x $$.

- For example, when $$ x = 2 $$, the equation gives us $$ y = 3 \cdot 2^2 = 3 \cdot 4 = 12 $$, which matches our table.

Now, let's sketch a graph for this:

- When $$ x = -1 $$, $$ y = 1.5 $$.
- When $$ x = 0 $$, $$ y = 3 $$.
- When $$ x = 1 $$, $$ y = 6 $$.
- When $$ x = 2 $$, $$ y = 12 $$.

You'll see a curve going up fast as $$ x $$ increases, and it gets closer to the x-axis as $$ x $$ decreases. This is what exponential growth looks like!

Next, letâ€™s talk about exponential decay. Imagine a table like before:

| x | y |
|---|---|
| 0 | 3 |
| 1 | 1.5 |
| 2 | 0.75 |
| -1 | 6 |

Now, when $$ x = 0 $$, $$ y = 3 $$ again. But this time, every time we increase $$ x $$ by 1, we multiply $$ y $$ by $$ \frac{1}{2} $$:

- When $$ x = 1 $$, $$ y = \frac{3}{2} $$ or 1.5.
- When $$ x = 2 $$, $$ y = \frac{3}{4} $$ or 0.75.

For negative $$ x $$ values:

- When $$ x = -1 $$, $$ y = 6 $$.

The equation for this would be: $$ y = 3 \cdot \left(\frac{1}{2}\right)^x $$.

- For example, when $$ x = 1 $$, the equation gives us $$ y = 3 \cdot \left(\frac{1}{2}\right) = 1.5 $$, which matches our table.

When graphed:

- When $$ x = -1 $$, $$ y = 6 $$.
- When $$ x = 0 $$, $$ y = 3 $$.
- When $$ x = 1 $$, $$ y = 1.5 $$.
- When $$ x = 2 $$, $$ y = 0.75 $$.

You'll notice the curve gets closer to the x-axis as $$ x $$ increases, showing that the values shrink but never quite reach zero.

To sum up, equations look like this for both:

- **Exponential growth**: $$ y = A \cdot r^x $$ with $$ |r| > 1 $$.
- **Exponential decay**: $$ y = A \cdot r^x $$ with $$ |r| < 1 $$.

If $$ r = 1 $$, the equation becomes a flat line: $$ y = A $$.

Hope this makes sense! Feel free to ask me any questions if you're curious about any part of this topic.