Hey there! Let's go through this together and figure out how to eliminate a variable in a system of equations. Hereâ€™s what you need to do:

**Question 1:**
- **Strategy A:** Add the equations
  - Let's try adding them:
    $$
    \begin{aligned}
    5x + 5x &= 10x \\
    -3y + 4y &= y \\
    -3 + 6 &= 3
    \end{aligned}
    $$
    See? We get a new equation: $$10x + y = 3$$. No variables are eliminated here, so this strategy doesn't work.

- **Strategy B:** Subtract the bottom equation from the top
  - Let's try subtracting:
    $$
    \begin{aligned}
    5x - 5x &= 0 \\
    -3y - 4y &= -7y \\
    -3 - 6 &= -9
    \end{aligned}
    $$
    This results in $$-7y = -9$$, which shows weâ€™ve eliminated $$x$$! So, this strategy works.

- **Strategy C:** Multiply the top equation by 2, then add the equations
  - Let's first multiply the top equation by 2:
    $$
    10x - 6y = -6
    $$
  - Now, add the equations:
    $$
    \begin{aligned}
    10x + 5x &= 15x \\
    -6y + 4y &= -2y
    \end{aligned}
    $$
    This gives us $$15x - 2y$$, which doesn't eliminate any variables. So, this strategy doesn't work either.

**Question 2:**
- **Strategy A:** Multiply the bottom equation by 2, then add the equations
  - First, multiply:
    $$
    \begin{aligned}
    2x - 4y &= 10 \\
    \end{aligned}
    $$
  - Now, add:
    $$
    \begin{aligned}
    4x + 2x &= 6x \\
    4y - 4y &= 0
    \end{aligned}
    $$
    We get $$6x = ...$$ and $$0$$. This eliminates the $$y$$ variable, so this strategy works.

- **Strategy B:** Multiply the bottom equation by 4, then subtract it from the top
  - Multiply first:
    $$
    \begin{aligned}
    4x - 8y &= 20 \\
    \end{aligned}
    $$
  - Now, subtract:
    $$
    \begin{aligned}
    4x - 4x &= 0 \\
    4y - (-8y) &= 12y \\
    -2 - 20 &= -22
    \end{aligned}
    $$
    We end up with $$12y = -22$$ and zero $$x$$. So, this strategy eliminates $$x$$, and it works too.

- **Strategy C:** Multiply the top equation by 1/2, then add the equations
  - First, multiply:
    $$
    \begin{aligned}
    2x + 2y &= -1 \\
    \end{aligned}
    $$
  - Now, add:
    $$
    \begin{aligned}
    2x + x &= 3x \\
    2y - 2y &= 0
    \end{aligned}
    $$
    This gives us $$3x$$ and the $$0$$, which eliminates $$y$$. So this strategy works.

This was pretty fun, right? You can see there are many ways to tackle these systems, and understanding these options makes solving them easier!

Let's keep working on these skills. Ready for another example? 

**Next Example:**
- **Strategy A:** Subtract the bottom equation from the top
  - Let's subtract:
    $$
    \begin{aligned}
    3x - (-2x) &= 5x \\
    -3y - 4y &= -7y
    \end{aligned}
    $$
    We get $$5x - 7y$$, and no variables are eliminated. So this strategy doesnâ€™t work.

- **Strategy B:** Multiply the top equation by 3, and the bottom equation by 2, then add the equations
  - Multiplying:
    $$
    \begin{aligned}
    9x - 9y &= 21 \\
    -4x + 8y &= 14
    \end{aligned}
    $$
  - Now, add:
    $$
    \begin{aligned}
    9x - 4x &= 5x \\
    -9y + 8y &= -y
    \end{aligned}
    $$
    This gives us $$5x - y$$, and no variables are eliminated. So this strategy doesnâ€™t work either.

- **Strategy C:** Multiply the top equation by 2, and the bottom equation by 3, then add the equations
  - Multiplying:
    $$
    \begin{aligned}
    6x - 6y &= 14 \\
    -6x + 12y &= 21
    \end{aligned}
    $$
  - Now, add:
    $$
    \begin{aligned}
    6x - 6x &= 0 \\
    -6y + 12y &= 6y
    \end{aligned}
    $$
    We get $$0$$ and $$6y = ...$$. This eliminates the $$x$$ variable. So this strategy works.

Great job! Keep practicing to get better and more comfortable with these strategies. You've got this! ðŸ˜Š