Sure, let's break it down step by step!

We have the equation \( 20 - 7x = 6x - 6 \). We need to find the value of \( x \).

First, we'll move the constant terms (20 and -6) to one side of the equation, and the \( x \) terms (-7x and 6x) to the other side. Let's put the constants on the right side and the \( x \) terms on the left side.

To move the 20 from the left side, we subtract it from both sides. Remember, in an equation, whatever you do to one side, you must do to the other side to keep it balanced.

So, we subtract 20 from both sides:

\[ 20 - 7x - 20 = 6x - 6 - 20 \]

This simplifies to:

\[ -7x = 6x - 26 \]

Next, we want to get all the \( x \) terms on the left side. To do this, we'll subtract 6x from both sides:

\[ -7x - 6x = 6x - 26 - 6x \]

Which simplifies to:

\[ -13x = -26 \]

Now, we need to isolate \( x \). Currently, it is multiplied by -13. To isolate it, we divide both sides of the equation by -13:

\[ \frac{-13x}{-13} = \frac{-26}{-13} \]

This simplifies to:

\[ x = 2 \]

So, \( x = 2 \) is our answer.

Let's check to make sure it's correct by plugging it back into the original equation:

The original equation is:

\[ 20 - 7x = 6x - 6 \]

Substitute \( x = 2 \):

\[ 20 - 7(2) = 6(2) - 6 \]

Simplify both sides:

\[ 20 - 14 = 12 - 6 \]

Which simplifies to:

\[ 6 = 6 \]

Both sides are equal, so our solution \( x = 2 \) is correct! Great job!