Hey! Let's work together to solve this problem. We have a geometric sequence, and the formula for this sequence is given by:

$$A_i = 3 \left( -\frac{1}{4} \right)^{i-1}$$

Our goal is to find the fifth term in the sequence, denoted as $$A_5$$.

So, let's use the formula and plug in $$i = 5$$:

$$A_5 = 3 \left( -\frac{1}{4} \right)^{5-1}$$

Which simplifies to:

$$A_5 = 3 \left( -\frac{1}{4} \right)^4$$

Now, let's calculate $$\left( -\frac{1}{4} \right)^4$$. When we raise a negative number to an even power, the result will be positive because a negative multiplied by itself an even number of times becomes positive. So, we have:

$$\left( -\frac{1}{4} \right)^4 = \left( \frac{1}{4} \right)^4$$

Next, we compute $$\left( \frac{1}{4} \right)^4$$:

$$\left( \frac{1}{4} \right)^4 = \frac{1^4}{4^4} = \frac{1}{256}$$

Finally, we multiply this result by 3:

$$A_5 = 3 \times \frac{1}{256} = \frac{3}{256}$$

So, the fifth term in our sequence is:

$$\boxed{\frac{3}{256}}$$

There we go! We found the fifth term, and it's $$\frac{3}{256}$$. Nice job!