Sure, let's go through this together in a simple way:

We start with the equation: 

$$-9 - (9x - 6) = 3 \times (4x + 6) $$

First, we get rid of the parentheses by multiplying through. Notice that having a minus sign in front of the parentheses is like having a -1 being multiplied by what's inside. Similarly, we multiply on the right side by 3, using the distributive property.

So, let's do that:

$$-9 - 1 \times (9x - 6) = 3 \times (4x + 6) $$

Breaking it down, we get:

$$-9 - 9x + 6 = 12x + 18$$

Notice that -1 times 9x is -9x, and -1 times -6 is +6. On the right side, 3 times 4x is 12x, and 3 times 6 is 18.

Next, we combine like terms on the left side:

$$-9 + 6 - 9x = 12x + 18$$

So, -9 plus 6 is -3. Now we have:

$$-9x - 3 = 12x + 18$$

Now, we want to move all the $$x$$ terms to one side and the constants (numbers without $$x$$) to the other side. I prefer to move $$x$$ terms to the left, but you can do it the other way if you like.

To do that, we subtract $$12x$$ from both sides:

$$-9x - 3 - 12x = 12x + 18 - 12x$$

This simplifies to:

$$-21x - 3 = 18$$

Next, we need to move the number -3 to the other side by adding 3 to both sides:

$$-21x - 3 + 3 = 18 + 3$$

This leaves us with:

$$-21x = 21$$

To solve for $$x$$, we divide both sides by -21:

$$x = \frac{21}{-21}$$

Which means:

$$x = -1$$

Now, let's check our work by plugging $$x = -1$$ back into the original equation. 

For the left side:

$$-9 - (9 \times -1 - 6) = -9 - (-9 - 6) = -9 - (-15) = -9 + 15 = 6$$

For the right side:

$$3 \times (4 \times -1 + 6) = 3 \times (-4 + 6) = 3 \times 2 = 6$$

Both sides equal 6, so our solution $$x = -1$$ is correct. 

Great job! If you have any more questions, feel free to ask!