Sure! Let's go through this step-by-step together. We're given that $$b(1) = -7$$ and $$b(n) = b(n - 1) + 12$$. Our goal is to find the fourth term, $$b(4)$$, in the sequence.

First, let's break this down:

1. We know $$b(1)$$ is $$-7$$. So, we start there.
2. To find $$b(2)$$, we use the formula: $$b(2) = b(1) + 12$$.
3. To find $$b(3)$$, we then use: $$b(3) = b(2) + 12$$.
4. Finally, to find $$b(4)$$, we use: $$b(4) = b(3) + 12$$.

Letâ€™s work it out step-by-step:

- We know $$b(1) = -7$$.

Using this information:

- $$b(2) = b(1) + 12 = -7 + 12 = 5$$.

With $$b(2)$$:

- $$b(3) = b(2) + 12 = 5 + 12 = 17$$.

And finally, with $$b(3)$$:

- $$b(4) = b(3) + 12 = 17 + 12 = 29$$.

So, the fourth term, $$b(4)$$, is 29. Great job following along!